add single timestamp parser comparison

deps/poulet4/lib/P4automata/Benchmarks/Timestamp.v
@@ -17,6 +17,431 @@ Ltac prep_equiv :=
 
 Obligation Tactic := prep_equiv.
 
+Module TimestampRefSingle.
+  Inductive state :=
+  | Start
+  | ParseValue1
+  | ParseValue2
+  | ParseValue3
+  | ParseValue4
+  | ParseValue5
+  | ParseValue6.
+
+  Scheme Equality for state.
+
+  Global Instance state_eqdec: EquivDec.EqDec state eq := state_eq_dec.
+  Global Program Instance state_finite: @Finite state _ state_eq_dec :=
+    {| enum := [Start; ParseValue1; ParseValue2; ParseValue3; ParseValue4; ParseValue5; ParseValue6] |}.
+  Next Obligation.
+    repeat constructor;
+      repeat match goal with
+            | H: List.In _ [] |- _ => apply List.in_nil in H; exfalso; exact H
+            | |- ~ List.In _ [] => apply List.in_nil
+            | |- ~ List.In _ (_ :: _) => unfold not; intros
+            | H: List.In _ (_::_) |- _ => inversion H; clear H
+            | _ => discriminate
+            end.
+  Qed.
+  Next Obligation.
+    destruct x; intuition congruence.
+  Qed.
+
+  Inductive header : nat -> Type :=
+  | Typ : header 8
+  | Len : header 8
+  | Value : header 48
+  | Scratch8 : header 8
+  | Scratch16 : header 16
+  | Scratch24 : header 24
+  | Scratch32 : header 32
+  | Scratch40 : header 40.
+
+  Derive Signature for header.
+
+  Definition h16_eq_dec (x y: header 16) : {x = y} + {x <> y} :=
+    match x, y with 
+    | Scratch16, Scratch16 => left eq_refl
+    | _, _ => idProp
+    end.
+
+  Definition h24_eq_dec (x y: header 24) : {x = y} + {x <> y} :=
+    match x, y with 
+    | Scratch24, Scratch24 => left eq_refl
+    | _, _ => idProp
+    end.
+
+  Definition h32_eq_dec (x y: header 32) : {x = y} + {x <> y} :=
+    match x, y with 
+    | Scratch32, Scratch32 => left eq_refl
+    | _, _ => idProp
+    end.
+
+  Definition h40_eq_dec (x y: header 40) : {x = y} + {x <> y} :=
+    match x, y with 
+    | Scratch40, Scratch40 => left eq_refl
+    | _, _ => idProp
+    end.
+
+  Definition h48_eq_dec (x y: header 48) : {x = y} + {x <> y} :=
+    match x, y with 
+    | Value, Value => left eq_refl
+    | _, _ => idProp
+    end.
+
+  Definition h8_eq_dec (x y: header 8) : {x = y} + {x <> y}. 
+  refine (
+    match x with 
+    | Typ => 
+      match y with 
+      | Typ => left eq_refl
+      | Len => right _
+      | Scratch8 => right _
+      end
+    | Len => 
+      match y with 
+      | Typ => right _
+      | Len => left eq_refl
+      | Scratch8 => right _
+      end
+    | Scratch8 => 
+        match y with 
+        | Typ => right _
+        | Len => right _
+        | Scratch8 => left eq_refl
+        end
+    end
+  ); unfold "<>"; intros H; inversion H.
+  Defined.
+
+
+  Definition header_eqdec_ (n: nat) (x: header n) (y: header n) : {x = y} + {x <> y}.
+    solve_header_eqdec_ n x y 
+      ((existT (fun n => forall x y: header n, {x = y} + {x <> y}) _ h8_eq_dec) :: 
+        (existT _ _ h16_eq_dec) :: (existT _ _ h24_eq_dec) :: (existT _ _ h32_eq_dec) :: 
+        (existT _ _ h40_eq_dec) :: (existT _ _ h48_eq_dec) :: nil).
+  Defined. 
+
+  Global Instance header_eqdec: forall n, EquivDec.EqDec (header n) eq := header_eqdec_.
+
+  Global Instance header_eqdec': EquivDec.EqDec (Syntax.H' header) eq.
+  Proof.
+    solve_eqdec'.
+  Defined.
+
+  Global Instance header_finite: forall n, @Finite (header n) _ _.
+  Proof.
+    intros n; solve_indexed_finiteness n [8; 16; 24; 32; 40; 48].
+  Qed.
+
+  Global Program Instance header_finite': @Finite {n & header n} _ header_eqdec' :=
+    {| enum := [ 
+      existT _ _ Len; existT _ _ Typ; existT _ _ Value;  
+      existT _ _ Scratch8; existT _ _ Scratch16; existT _ _ Scratch24;
+      existT _ _ Scratch32; existT _ _ Scratch40
+      
+      ] |}.
+  Next Obligation.
+    solve_header_finite.
+  Qed.
+  Next Obligation.
+  dependent destruction X; subst;
+  repeat (
+    match goal with
+    | |- ?L \/ ?R => (now left; trivial) || right
+    end
+  ).
+  Qed.
+
+  Definition states (s: state) :=
+    match s with
+    | Start =>
+      {| st_op := 
+          extract(Typ) ;;
+          extract(Len) ;
+        st_trans := transition select (| EHdr Len |) {{
+          [| exact #b|0|0|0|0|0|0|0|0 |] ==> accept ;;;
+          [| exact #b|0|0|0|0|0|0|0|1 |] ==> inl ParseValue1 ;;;
+          [| exact #b|0|0|0|0|0|0|1|0 |] ==> inl ParseValue2 ;;;
+          [| exact #b|0|0|0|0|0|0|1|1 |] ==> inl ParseValue3 ;;;
+          [| exact #b|0|0|0|0|0|1|0|0 |] ==> inl ParseValue4 ;;;
+          [| exact #b|0|0|0|0|0|1|0|1 |] ==> inl ParseValue5 ;;;
+          [| exact #b|0|0|0|0|0|1|1|0 |] ==> inl ParseValue6 ;;;
+            reject
+        }}
+      |}
+    | ParseValue1 =>
+      {| st_op := 
+          extract(Scratch8) ;; 
+          Value <- EConcat (m := 40) (EHdr Scratch8) ((EHdr Value)[48--8])  ;
+        st_trans := transition accept
+      |}
+    | ParseValue2 =>
+      {| st_op := 
+          extract(Scratch16) ;; 
+          Value <- EConcat (m := 32) (EHdr Scratch16) ((EHdr Value)[48--16])  ;
+        st_trans := transition accept
+      |}
+    | ParseValue3 =>
+      {| st_op := 
+          extract(Scratch24) ;; 
+          Value <- EConcat (m := 24) (EHdr Scratch24) ((EHdr Value)[48--24])  ;
+        st_trans := transition accept
+      |}
+    | ParseValue4 =>
+      {| st_op := 
+          extract(Scratch32) ;; 
+          Value <- EConcat (m := 16) (EHdr Scratch32) ((EHdr Value)[48--32])  ;
+        st_trans := transition accept
+      |}
+    | ParseValue5 =>
+      {| st_op := 
+          extract(Scratch40) ;; 
+          Value <- EConcat (m := 8) (EHdr Scratch40) ((EHdr Value)[48--40])  ;
+        st_trans := transition accept
+      |}
+    | ParseValue6 =>
+      {| st_op := extract(Value) ;
+        st_trans := transition accept
+      |}
+    end.
+
+  Program Definition aut: Syntax.t state header :=
+    {| t_states := states |}.
+  Solve Obligations with (destruct s; cbv; Lia.lia).
+
+End TimestampRefSingle.
+
+
+Module TimestampSpecSingle.
+  Inductive state :=
+  | Start
+  | ParseValue1
+  | ParseValue2
+  | ParseValue3
+  | ParseValue4
+  | ParseValue5
+  | ParseValue6
+  | ParseTimestamp.
+
+  Scheme Equality for state.
+
+  Global Instance state_eqdec: EquivDec.EqDec state eq := state_eq_dec.
+  Global Program Instance state_finite: @Finite state _ state_eq_dec :=
+    {| enum := [Start; ParseValue1; ParseValue2; ParseValue3; ParseValue4; ParseValue5; ParseValue6; ParseTimestamp] |}.
+  Next Obligation.
+    repeat constructor;
+      repeat match goal with
+            | H: List.In _ [] |- _ => apply List.in_nil in H; exfalso; exact H
+            | |- ~ List.In _ [] => apply List.in_nil
+            | |- ~ List.In _ (_ :: _) => unfold not; intros
+            | H: List.In _ (_::_) |- _ => inversion H; clear H
+            | _ => discriminate
+            end.
+  Qed.
+  Next Obligation.
+    destruct x; intuition congruence.
+  Qed.
+
+  Inductive header : nat -> Type :=
+  | Typ : header 8
+  | Len : header 8
+  | Scratch8 : header 8
+  | Scratch16 : header 16
+  | Scratch24 : header 24
+  | Scratch32 : header 32
+  | Scratch40 : header 40
+  | Scratch48 : header 48
+  | Pointer : header 8
+  | Overflow: header 4
+  | Flag: header 4
+  | Timestamp: header 32.
+
+  Derive Signature for header.
+
+  Definition h4_eq_dec (x y: header 4) : {x = y} + {x <> y}.
+  refine (
+    match x, y with
+    | Overflow, Flag => right _
+    | Flag, Overflow => right _ 
+    | Flag, Flag => left eq_refl
+    | Overflow, Overflow => left eq_refl
+    end
+  ); unfold "<>"; intros H; inversion H.
+  Defined.
+
+  Definition h16_eq_dec (x y: header 16) : {x = y} + {x <> y} :=
+    match x, y with 
+    | Scratch16, Scratch16 => left eq_refl
+    | _, _ => idProp
+    end.
+
+  Definition h24_eq_dec (x y: header 24) : {x = y} + {x <> y} :=
+    match x, y with 
+    | Scratch24, Scratch24 => left eq_refl
+    | _, _ => idProp
+    end.
+
+  Definition h32_eq_dec (x y: header 32) : {x = y} + {x <> y}.
+  refine (
+    match x, y with
+    | Scratch32, Timestamp => right _
+    | Timestamp, Scratch32 => right _ 
+    | Timestamp, Timestamp => left eq_refl
+    | Scratch32, Scratch32 => left eq_refl
+    end
+  ); unfold "<>"; intros H; inversion H.
+  Defined.
+
+
+  Definition h40_eq_dec (x y: header 40) : {x = y} + {x <> y} :=
+    match x, y with 
+    | Scratch40, Scratch40 => left eq_refl
+    | _, _ => idProp
+    end.
+
+  Definition h48_eq_dec (x y: header 48) : {x = y} + {x <> y} :=
+    match x, y with 
+    | Scratch48, Scratch48 => left eq_refl
+    | _, _ => idProp
+    end.
+
+  Definition h8_eq_dec (x y: header 8) : {x = y} + {x <> y}. 
+  refine (
+    match x with 
+    | Typ => 
+      match y with 
+      | Typ => left eq_refl
+      | Len => right _
+      | Scratch8 => right _
+      | Pointer => right _
+      end
+    | Len => 
+      match y with 
+      | Typ => right _
+      | Len => left eq_refl
+      | Scratch8 => right _
+      | Pointer => right _
+      end
+    | Scratch8 => 
+        match y with 
+        | Typ => right _
+        | Len => right _
+        | Scratch8 => left eq_refl
+        | Pointer => right _
+        end
+    | Pointer => 
+      match y with 
+      | Typ => right _
+      | Len => right _
+      | Scratch8 => right _
+      | Pointer => left eq_refl
+      end
+    end
+  ); unfold "<>"; intros H; inversion H.
+  Defined.
+
+
+  Definition header_eqdec_ (n: nat) (x: header n) (y: header n) : {x = y} + {x <> y}.
+    solve_header_eqdec_ n x y 
+      ((existT (fun n => forall x y: header n, {x = y} + {x <> y}) _ h8_eq_dec) :: 
+        (existT _ _ h16_eq_dec) :: (existT _ _ h24_eq_dec) :: (existT _ _ h32_eq_dec) :: 
+        (existT _ _ h40_eq_dec) :: (existT _ _ h48_eq_dec) :: (existT _ _ h4_eq_dec) :: nil).
+  Defined. 
+
+  Global Instance header_eqdec: forall n, EquivDec.EqDec (header n) eq := header_eqdec_.
+
+  Global Instance header_eqdec': EquivDec.EqDec (Syntax.H' header) eq.
+  Proof.
+    solve_eqdec'.
+  Defined.
+
+  Global Instance header_finite: forall n, @Finite (header n) _ _.
+  Proof.
+    intros n; solve_indexed_finiteness n [4; 8; 16; 24; 32; 40; 48].
+  Qed.
+
+  Global Program Instance header_finite': @Finite {n & header n} _ header_eqdec' :=
+    {| enum := [ 
+      existT _ _ Len; existT _ _ Typ;
+      existT _ _ Scratch8; existT _ _ Scratch16; existT _ _ Scratch24;
+      existT _ _ Scratch32; existT _ _ Scratch40; existT _ _ Scratch48;
+      existT _ _ Overflow; existT _ _ Flag; existT _ _ Pointer; existT _ _ Timestamp
+      ] |}.
+  Next Obligation.
+    solve_header_finite.
+  Qed.
+  Next Obligation.
+  dependent destruction X; subst;
+  repeat (
+    match goal with
+    | |- ?L \/ ?R => (now left; trivial) || right
+    end
+  ).
+  Qed.
+
+  Definition states (s: state) :=
+    match s with
+    | Start =>
+      {| st_op := 
+          extract(Typ) ;;
+          extract(Len) ;
+        st_trans := transition select (| EHdr Typ, EHdr Len |) {{
+          [| exact #b|0|1|0|0|0|1|0|0, exact #b|0|0|0|0|0|1|1|0 |] ==> inl ParseTimestamp ;;;
+          [| *, exact #b|0|0|0|0|0|0|0|0 |] ==> accept ;;;
+          [| *, exact #b|0|0|0|0|0|0|0|1 |] ==> inl ParseValue1 ;;;
+          [| *, exact #b|0|0|0|0|0|0|1|0 |] ==> inl ParseValue2 ;;;
+          [| *, exact #b|0|0|0|0|0|0|1|1 |] ==> inl ParseValue3 ;;;
+          [| *, exact #b|0|0|0|0|0|1|0|0 |] ==> inl ParseValue4 ;;;
+          [| *, exact #b|0|0|0|0|0|1|0|1 |] ==> inl ParseValue5 ;;;
+          [| *, exact #b|0|0|0|0|0|1|1|0 |] ==> inl ParseValue6 ;;;
+            reject
+        }}
+      |}
+    | ParseTimestamp =>
+      {| st_op := 
+          extract(Pointer) ;;
+          extract(Overflow) ;;
+          extract(Flag) ;;
+          extract(Timestamp) ;
+        st_trans := transition accept (* TODO: validate pointer and flag? *)
+      |}
+    | ParseValue1 =>
+      {| st_op := 
+          extract(Scratch8) ;
+        st_trans := transition accept
+      |}
+    | ParseValue2 =>
+      {| st_op := 
+          extract(Scratch16) ;
+        st_trans := transition accept
+      |}
+    | ParseValue3 =>
+      {| st_op := 
+          extract(Scratch24) ;
+        st_trans := transition accept
+      |}
+    | ParseValue4 =>
+      {| st_op := 
+          extract(Scratch32) ;
+        st_trans := transition accept
+      |}
+    | ParseValue5 =>
+      {| st_op := 
+          extract(Scratch40) ;
+        st_trans := transition accept
+      |}
+    | ParseValue6 =>
+      {| st_op := extract(Scratch48) ;
+        st_trans := transition accept
+      |}
+    end.
+
+  Program Definition aut: Syntax.t state header :=
+    {| t_states := states |}.
+  Solve Obligations with (destruct s; cbv; Lia.lia).
+
+End TimestampSpecSingle.
+
 
 Module TimestampRefSmall.
   Inductive state :=
